src/out/Test.ml
@@ -1,5 +1,5 @@
 open Prims
-let (bc_0x7f92191c0c90 : Structs.bytecode) =
+let (bc_0x7f2c2b61cdf0 : Structs.bytecode) =
   Structs.CODE
     [Structs.LOAD_CONST Prims.int_one;
     Structs.LOAD_CONST (Prims.of_int (2));
@@ -9,62 +9,198 @@ let (bc_0x7f92191c0c90 : Structs.bytecode) =
     Structs.LOAD_CONST (Prims.of_int (4));
     Structs.MAKE_FUNCTION Prims.int_zero;
     Structs.STORE_FAST Prims.int_one;
+    Structs.LOAD_CONST (Prims.of_int (5));
+    Structs.LOAD_CONST (Prims.of_int (6));
+    Structs.MAKE_FUNCTION Prims.int_zero;
+    Structs.STORE_FAST (Prims.of_int (2));
     Structs.LOAD_FAST Prims.int_zero;
     Structs.CALL_FUNCTION Prims.int_zero;
     Structs.LOAD_FAST Prims.int_one;
     Structs.CALL_FUNCTION Prims.int_zero;
-    Structs.BINARY_MULTIPLY;
+    Structs.LOAD_FAST (Prims.of_int (2));
+    Structs.CALL_FUNCTION Prims.int_zero;
+    Structs.BUILD_LIST (Prims.of_int (3));
+    Structs.STORE_FAST (Prims.of_int (3));
+    Structs.LOAD_FAST (Prims.of_int (3));
     Structs.RETURN_VALUE]
-let (bc_0x7f92191c0be0 : Structs.bytecode) =
-  Structs.CODE [Structs.LOAD_CONST Prims.int_one; Structs.RETURN_VALUE]
-let (consts_0x7f92191c0be0 : Structs.pyObj Prims.list) =
+let (bc_0x7f2c2b61cd40 : Structs.bytecode) =
+  Structs.CODE
+    [Structs.LOAD_CONST Prims.int_one;
+    Structs.STORE_FAST Prims.int_zero;
+    Structs.LOAD_CONST (Prims.of_int (2));
+    Structs.STORE_FAST Prims.int_one;
+    Structs.LOAD_CONST Prims.int_one;
+    Structs.STORE_FAST (Prims.of_int (2));
+    Structs.LOAD_CONST (Prims.of_int (2));
+    Structs.STORE_FAST (Prims.of_int (3));
+    Structs.LOAD_CONST (Prims.of_int (2));
+    Structs.STORE_FAST (Prims.of_int (4));
+    Structs.LOAD_CONST Prims.int_one;
+    Structs.STORE_FAST (Prims.of_int (5));
+    Structs.BUILD_LIST Prims.int_zero;
+    Structs.UNARY_NOT;
+    Structs.STORE_FAST (Prims.of_int (6));
+    Structs.LOAD_CONST (Prims.of_int (3));
+    Structs.BUILD_LIST Prims.int_one;
+    Structs.UNARY_NOT;
+    Structs.STORE_FAST (Prims.of_int (7));
+    Structs.LOAD_CONST Prims.int_one;
+    Structs.STORE_FAST (Prims.of_int (8));
+    Structs.LOAD_CONST (Prims.of_int (2));
+    Structs.STORE_FAST (Prims.of_int (9));
+    Structs.BUILD_MAP Prims.int_zero;
+    Structs.UNARY_NOT;
+    Structs.STORE_FAST (Prims.of_int (10));
+    Structs.LOAD_CONST (Prims.of_int (3));
+    Structs.LOAD_CONST (Prims.of_int (4));
+    Structs.BUILD_MAP Prims.int_one;
+    Structs.UNARY_NOT;
+    Structs.STORE_FAST (Prims.of_int (11));
+    Structs.LOAD_CONST Prims.int_one;
+    Structs.STORE_FAST (Prims.of_int (12));
+    Structs.LOAD_FAST Prims.int_zero;
+    Structs.LOAD_FAST Prims.int_one;
+    Structs.LOAD_FAST (Prims.of_int (2));
+    Structs.LOAD_FAST (Prims.of_int (3));
+    Structs.LOAD_FAST (Prims.of_int (4));
+    Structs.LOAD_FAST (Prims.of_int (5));
+    Structs.LOAD_FAST (Prims.of_int (6));
+    Structs.LOAD_FAST (Prims.of_int (7));
+    Structs.LOAD_FAST (Prims.of_int (8));
+    Structs.LOAD_FAST (Prims.of_int (9));
+    Structs.LOAD_FAST (Prims.of_int (10));
+    Structs.LOAD_FAST (Prims.of_int (11));
+    Structs.LOAD_FAST (Prims.of_int (12));
+    Structs.BUILD_TUPLE (Prims.of_int (13));
+    Structs.RETURN_VALUE]
+let (consts_0x7f2c2b61cd40 : Structs.pyObj Prims.list) =
   [Structs.PYTYP (PyNone.createNone ());
-  Structs.PYTYP (PyInt.createInt (Prims.of_int (3)))]
-let varnames_0x7f92191c0be0 : 'uuuuu . unit -> 'uuuuu Prims.list =
+  Structs.PYTYP (PyBool.createBool true);
+  Structs.PYTYP (PyBool.createBool false);
+  Structs.PYTYP (PyInt.createInt Prims.int_one);
+  Structs.PYTYP (PyInt.createInt (Prims.of_int (2)))]
+let (varnames_0x7f2c2b61cd40 : Prims.string Prims.list) =
+  ["x11";
+  "x12";
+  "x21";
+  "x22";
+  "x31";
+  "x32";
+  "x41";
+  "x42";
+  "x51";
+  "x52";
+  "x61";
+  "x62";
+  "x7"]
+let names_0x7f2c2b61cd40 : 'uuuuu . unit -> 'uuuuu Prims.list =
   fun uu___ -> []
-let names_0x7f92191c0be0 : 'uuuuu . unit -> 'uuuuu Prims.list =
-  fun uu___ -> []
-let (co_0x7f92191c0be0 : Structs.codeObj) =
+let (co_0x7f2c2b61cd40 : Structs.codeObj) =
   {
-    Structs.co_code = bc_0x7f92191c0be0;
-    Structs.co_consts = consts_0x7f92191c0be0;
-    Structs.co_varnames = (varnames_0x7f92191c0be0 ());
-    Structs.co_names = (names_0x7f92191c0be0 ())
+    Structs.co_code = bc_0x7f2c2b61cd40;
+    Structs.co_consts = consts_0x7f2c2b61cd40;
+    Structs.co_varnames = varnames_0x7f2c2b61cd40;
+    Structs.co_names = (names_0x7f2c2b61cd40 ())
   }
-let (bc_0x7f92191c0a80 : Structs.bytecode) =
-  Structs.CODE [Structs.LOAD_CONST Prims.int_one; Structs.RETURN_VALUE]
-let (consts_0x7f92191c0a80 : Structs.pyObj Prims.list) =
+let (bc_0x7f2c2b61cc90 : Structs.bytecode) =
+  Structs.CODE
+    [Structs.LOAD_CONST Prims.int_one;
+    Structs.STORE_FAST Prims.int_zero;
+    Structs.LOAD_FAST Prims.int_zero;
+    Structs.LOAD_CONST (Prims.of_int (2));
+    Structs.INPLACE_SUBTRACT;
+    Structs.STORE_FAST Prims.int_zero;
+    Structs.LOAD_FAST Prims.int_zero;
+    Structs.RETURN_VALUE]
+let (consts_0x7f2c2b61cc90 : Structs.pyObj Prims.list) =
   [Structs.PYTYP (PyNone.createNone ());
-  Structs.PYTYP (PyInt.createInt (Prims.of_int (7)))]
-let varnames_0x7f92191c0a80 : 'uuuuu . unit -> 'uuuuu Prims.list =
+  Structs.PYTYP (PyInt.createInt (Prims.of_int (2)));
+  Structs.PYTYP (PyInt.createInt Prims.int_one)]
+let (varnames_0x7f2c2b61cc90 : Prims.string Prims.list) = ["x"]
+let names_0x7f2c2b61cc90 : 'uuuuu . unit -> 'uuuuu Prims.list =
   fun uu___ -> []
-let names_0x7f92191c0a80 : 'uuuuu . unit -> 'uuuuu Prims.list =
-  fun uu___ -> []
-let (co_0x7f92191c0a80 : Structs.codeObj) =
+let (co_0x7f2c2b61cc90 : Structs.codeObj) =
   {
-    Structs.co_code = bc_0x7f92191c0a80;
-    Structs.co_consts = consts_0x7f92191c0a80;
-    Structs.co_varnames = (varnames_0x7f92191c0a80 ());
-    Structs.co_names = (names_0x7f92191c0a80 ())
+    Structs.co_code = bc_0x7f2c2b61cc90;
+    Structs.co_consts = consts_0x7f2c2b61cc90;
+    Structs.co_varnames = varnames_0x7f2c2b61cc90;
+    Structs.co_names = (names_0x7f2c2b61cc90 ())
   }
-let (consts_0x7f92191c0c90 : Structs.pyObj Prims.list) =
+let (bc_0x7f2c2b61cbe0 : Structs.bytecode) =
+  Structs.CODE
+    [Structs.LOAD_CONST Prims.int_one;
+    Structs.STORE_FAST Prims.int_zero;
+    Structs.LOAD_CONST (Prims.of_int (2));
+    Structs.BUILD_LIST Prims.int_one;
+    Structs.STORE_FAST Prims.int_one;
+    Structs.LOAD_CONST (Prims.of_int (2));
+    Structs.STORE_FAST (Prims.of_int (2));
+    Structs.LOAD_CONST (Prims.of_int (3));
+    Structs.STORE_FAST (Prims.of_int (3));
+    Structs.LOAD_FAST Prims.int_zero;
+    Structs.LOAD_CONST (Prims.of_int (2));
+    Structs.INPLACE_ADD;
+    Structs.STORE_FAST Prims.int_zero;
+    Structs.LOAD_FAST Prims.int_one;
+    Structs.LOAD_CONST (Prims.of_int (4));
+    Structs.BUILD_LIST Prims.int_one;
+    Structs.INPLACE_ADD;
+    Structs.STORE_FAST Prims.int_one;
+    Structs.LOAD_FAST (Prims.of_int (2));
+    Structs.LOAD_CONST (Prims.of_int (4));
+    Structs.INPLACE_ADD;
+    Structs.STORE_FAST (Prims.of_int (2));
+    Structs.LOAD_FAST (Prims.of_int (3));
+    Structs.LOAD_CONST (Prims.of_int (5));
+    Structs.INPLACE_ADD;
+    Structs.STORE_FAST (Prims.of_int (3));
+    Structs.LOAD_FAST Prims.int_zero;
+    Structs.LOAD_FAST Prims.int_one;
+    Structs.LOAD_FAST (Prims.of_int (2));
+    Structs.LOAD_FAST (Prims.of_int (3));
+    Structs.BUILD_TUPLE (Prims.of_int (4));
+    Structs.RETURN_VALUE]
+let (consts_0x7f2c2b61cbe0 : Structs.pyObj Prims.list) =
   [Structs.PYTYP (PyNone.createNone ());
-  Structs.CODEOBJECT co_0x7f92191c0a80;
-  Structs.PYTYP (PyString.createString "top_level.<locals>.test");
-  Structs.CODEOBJECT co_0x7f92191c0be0;
-  Structs.PYTYP (PyString.createString "top_level.<locals>.test2")]
-let (varnames_0x7f92191c0c90 : Prims.string Prims.list) = ["test"; "test2"]
-let names_0x7f92191c0c90 : 'uuuuu . unit -> 'uuuuu Prims.list =
+  Structs.PYTYP (PyInt.createInt Prims.int_zero);
+  Structs.PYTYP (PyInt.createInt Prims.int_one);
+  Structs.PYTYP (PyString.createString "");
+  Structs.PYTYP (PyInt.createInt (Prims.of_int (2)));
+  Structs.PYTYP (PyString.createString "1")]
+let (varnames_0x7f2c2b61cbe0 : Prims.string Prims.list) =
+  ["x1"; "x2"; "x3"; "x4"]
+let names_0x7f2c2b61cbe0 : 'uuuuu . unit -> 'uuuuu Prims.list =
   fun uu___ -> []
-let (co_0x7f92191c0c90 : Structs.codeObj) =
+let (co_0x7f2c2b61cbe0 : Structs.codeObj) =
   {
-    Structs.co_code = bc_0x7f92191c0c90;
-    Structs.co_consts = consts_0x7f92191c0c90;
-    Structs.co_varnames = varnames_0x7f92191c0c90;
-    Structs.co_names = (names_0x7f92191c0c90 ())
+    Structs.co_code = bc_0x7f2c2b61cbe0;
+    Structs.co_consts = consts_0x7f2c2b61cbe0;
+    Structs.co_varnames = varnames_0x7f2c2b61cbe0;
+    Structs.co_names = (names_0x7f2c2b61cbe0 ())
+  }
+let (consts_0x7f2c2b61cdf0 : Structs.pyObj Prims.list) =
+  [Structs.PYTYP (PyNone.createNone ());
+  Structs.CODEOBJECT co_0x7f2c2b61cbe0;
+  Structs.PYTYP
+    (PyString.createString "top_level.<locals>.test_UNARY_POSITIVE");
+  Structs.CODEOBJECT co_0x7f2c2b61cc90;
+  Structs.PYTYP
+    (PyString.createString "top_level.<locals>.test_UNARY_NEGATIVE");
+  Structs.CODEOBJECT co_0x7f2c2b61cd40;
+  Structs.PYTYP (PyString.createString "top_level.<locals>.test_UNARY_NOT")]
+let (varnames_0x7f2c2b61cdf0 : Prims.string Prims.list) =
+  ["test_UNARY_POSITIVE"; "test_UNARY_NEGATIVE"; "test_UNARY_NOT"; "result"]
+let names_0x7f2c2b61cdf0 : 'uuuuu . unit -> 'uuuuu Prims.list =
+  fun uu___ -> []
+let (co_0x7f2c2b61cdf0 : Structs.codeObj) =
+  {
+    Structs.co_code = bc_0x7f2c2b61cdf0;
+    Structs.co_consts = consts_0x7f2c2b61cdf0;
+    Structs.co_varnames = varnames_0x7f2c2b61cdf0;
+    Structs.co_names = (names_0x7f2c2b61cdf0 ())
   }
 let (uu___0 : (Structs.vm * Structs.pyObj)) =
-  VM.runCode_returnVM co_0x7f92191c0c90
+  VM.runCode_returnVM co_0x7f2c2b61cdf0
 let (virt_m : Structs.vm) = match uu___0 with | (virt_m1, res) -> virt_m1
 let (res : Structs.pyObj) = match uu___0 with | (virt_m1, res1) -> res1
 let (print_program_state : unit) =
