test/hand_crafted/binary_operations.py
@@ -1,0 +1,2 @@
+def top_level():
+    return 1 + 2
