test/hand_crafted/variables.py
@@ -1,3 +1,7 @@
-var_1 = 1
-var_2 = 2
-var_3 = var_1 * var_2
+def top_level():
+    var_1 = 1
+    var_2 = 2
+    var_3 = 3
+    var_4 = var_1 * var_2 * 3
+    
+    return var_1, var_2, var_3, var_4 
