src/test/Test.fst
@@ -7,7 +7,7 @@ open Utils
 open PyBuiltinObjects
 (* ---------------- *)
 
-let bc_0x7f92191c0c90 = CODE [
+let bc_0x7f2c2b61cdf0 = CODE [
   LOAD_CONST 1;
   LOAD_CONST 2;
   MAKE_FUNCTION 0;
@@ -16,82 +16,225 @@ let bc_0x7f92191c0c90 = CODE [
   LOAD_CONST 4;
   MAKE_FUNCTION 0;
   STORE_FAST 1;
+  LOAD_CONST 5;
+  LOAD_CONST 6;
+  MAKE_FUNCTION 0;
+  STORE_FAST 2;
   LOAD_FAST 0;
   CALL_FUNCTION 0;
   LOAD_FAST 1;
   CALL_FUNCTION 0;
-  BINARY_MULTIPLY ;
+  LOAD_FAST 2;
+  CALL_FUNCTION 0;
+  BUILD_LIST 3;
+  STORE_FAST 3;
+  LOAD_FAST 3;
   RETURN_VALUE ;
 ]
 
-let bc_0x7f92191c0be0 = CODE [
+let bc_0x7f2c2b61cd40 = CODE [
   LOAD_CONST 1;
-  RETURN_VALUE ;
-]
-
-let consts_0x7f92191c0be0 = [
-  PYTYP(createNone());
-  PYTYP(createInt 3);
-]
-
-let varnames_0x7f92191c0be0 = [
-]
-
-let names_0x7f92191c0be0 = [
-]
-
-let co_0x7f92191c0be0 = {
-  co_code = bc_0x7f92191c0be0;
-  co_consts = consts_0x7f92191c0be0;
-  co_varnames = varnames_0x7f92191c0be0;
-  co_names = names_0x7f92191c0be0
-}
-
-let bc_0x7f92191c0a80 = CODE [
+  STORE_FAST 0;
+  LOAD_CONST 2;
+  STORE_FAST 1;
   LOAD_CONST 1;
+  STORE_FAST 2;
+  LOAD_CONST 2;
+  STORE_FAST 3;
+  LOAD_CONST 2;
+  STORE_FAST 4;
+  LOAD_CONST 1;
+  STORE_FAST 5;
+  BUILD_LIST 0;
+  UNARY_NOT ;
+  STORE_FAST 6;
+  LOAD_CONST 3;
+  BUILD_LIST 1;
+  UNARY_NOT ;
+  STORE_FAST 7;
+  LOAD_CONST 1;
+  STORE_FAST 8;
+  LOAD_CONST 2;
+  STORE_FAST 9;
+  BUILD_MAP 0;
+  UNARY_NOT ;
+  STORE_FAST 10;
+  LOAD_CONST 3;
+  LOAD_CONST 4;
+  BUILD_MAP 1;
+  UNARY_NOT ;
+  STORE_FAST 11;
+  LOAD_CONST 1;
+  STORE_FAST 12;
+  LOAD_FAST 0;
+  LOAD_FAST 1;
+  LOAD_FAST 2;
+  LOAD_FAST 3;
+  LOAD_FAST 4;
+  LOAD_FAST 5;
+  LOAD_FAST 6;
+  LOAD_FAST 7;
+  LOAD_FAST 8;
+  LOAD_FAST 9;
+  LOAD_FAST 10;
+  LOAD_FAST 11;
+  LOAD_FAST 12;
+  BUILD_TUPLE 13;
   RETURN_VALUE ;
 ]
 
-let consts_0x7f92191c0a80 = [
+let consts_0x7f2c2b61cd40 = [
   PYTYP(createNone());
-  PYTYP(createInt 7);
+  PYTYP(createBool true);
+  PYTYP(createBool false);
+  PYTYP(createInt 1);
+  PYTYP(createInt 2);
 ]
 
-let varnames_0x7f92191c0a80 = [
+let varnames_0x7f2c2b61cd40 = [
+  "x11";
+  "x12";
+  "x21";
+  "x22";
+  "x31";
+  "x32";
+  "x41";
+  "x42";
+  "x51";
+  "x52";
+  "x61";
+  "x62";
+  "x7";
 ]
 
-let names_0x7f92191c0a80 = [
+let names_0x7f2c2b61cd40 = [
 ]
 
-let co_0x7f92191c0a80 = {
-  co_code = bc_0x7f92191c0a80;
-  co_consts = consts_0x7f92191c0a80;
-  co_varnames = varnames_0x7f92191c0a80;
-  co_names = names_0x7f92191c0a80
+let co_0x7f2c2b61cd40 = {
+  co_code = bc_0x7f2c2b61cd40;
+  co_consts = consts_0x7f2c2b61cd40;
+  co_varnames = varnames_0x7f2c2b61cd40;
+  co_names = names_0x7f2c2b61cd40
 }
 
-let consts_0x7f92191c0c90 = [
+let bc_0x7f2c2b61cc90 = CODE [
+  LOAD_CONST 1;
+  STORE_FAST 0;
+  LOAD_FAST 0;
+  LOAD_CONST 2;
+  INPLACE_SUBTRACT ;
+  STORE_FAST 0;
+  LOAD_FAST 0;
+  RETURN_VALUE ;
+]
+
+let consts_0x7f2c2b61cc90 = [
   PYTYP(createNone());
-  CODEOBJECT(co_0x7f92191c0a80);
-  PYTYP(createString "top_level.<locals>.test");
-  CODEOBJECT(co_0x7f92191c0be0);
-  PYTYP(createString "top_level.<locals>.test2");
+  PYTYP(createInt 2);
+  PYTYP(createInt 1);
 ]
 
-let varnames_0x7f92191c0c90 = [
-  "test";
-  "test2";
+let varnames_0x7f2c2b61cc90 = [
+  "x";
 ]
 
-let names_0x7f92191c0c90 = [
+let names_0x7f2c2b61cc90 = [
 ]
 
-let co_0x7f92191c0c90 = {
-  co_code = bc_0x7f92191c0c90;
-  co_consts = consts_0x7f92191c0c90;
-  co_varnames = varnames_0x7f92191c0c90;
-  co_names = names_0x7f92191c0c90
+let co_0x7f2c2b61cc90 = {
+  co_code = bc_0x7f2c2b61cc90;
+  co_consts = consts_0x7f2c2b61cc90;
+  co_varnames = varnames_0x7f2c2b61cc90;
+  co_names = names_0x7f2c2b61cc90
 }
 
-let virt_m, res = runCode_returnVM co_0x7f92191c0c90
+let bc_0x7f2c2b61cbe0 = CODE [
+  LOAD_CONST 1;
+  STORE_FAST 0;
+  LOAD_CONST 2;
+  BUILD_LIST 1;
+  STORE_FAST 1;
+  LOAD_CONST 2;
+  STORE_FAST 2;
+  LOAD_CONST 3;
+  STORE_FAST 3;
+  LOAD_FAST 0;
+  LOAD_CONST 2;
+  INPLACE_ADD ;
+  STORE_FAST 0;
+  LOAD_FAST 1;
+  LOAD_CONST 4;
+  BUILD_LIST 1;
+  INPLACE_ADD ;
+  STORE_FAST 1;
+  LOAD_FAST 2;
+  LOAD_CONST 4;
+  INPLACE_ADD ;
+  STORE_FAST 2;
+  LOAD_FAST 3;
+  LOAD_CONST 5;
+  INPLACE_ADD ;
+  STORE_FAST 3;
+  LOAD_FAST 0;
+  LOAD_FAST 1;
+  LOAD_FAST 2;
+  LOAD_FAST 3;
+  BUILD_TUPLE 4;
+  RETURN_VALUE ;
+]
+
+let consts_0x7f2c2b61cbe0 = [
+  PYTYP(createNone());
+  PYTYP(createInt 0);
+  PYTYP(createInt 1);
+  PYTYP(createString "");
+  PYTYP(createInt 2);
+  PYTYP(createString "1");
+]
+
+let varnames_0x7f2c2b61cbe0 = [
+  "x1";
+  "x2";
+  "x3";
+  "x4";
+]
+
+let names_0x7f2c2b61cbe0 = [
+]
+
+let co_0x7f2c2b61cbe0 = {
+  co_code = bc_0x7f2c2b61cbe0;
+  co_consts = consts_0x7f2c2b61cbe0;
+  co_varnames = varnames_0x7f2c2b61cbe0;
+  co_names = names_0x7f2c2b61cbe0
+}
+
+let consts_0x7f2c2b61cdf0 = [
+  PYTYP(createNone());
+  CODEOBJECT(co_0x7f2c2b61cbe0);
+  PYTYP(createString "top_level.<locals>.test_UNARY_POSITIVE");
+  CODEOBJECT(co_0x7f2c2b61cc90);
+  PYTYP(createString "top_level.<locals>.test_UNARY_NEGATIVE");
+  CODEOBJECT(co_0x7f2c2b61cd40);
+  PYTYP(createString "top_level.<locals>.test_UNARY_NOT");
+]
+
+let varnames_0x7f2c2b61cdf0 = [
+  "test_UNARY_POSITIVE";
+  "test_UNARY_NEGATIVE";
+  "test_UNARY_NOT";
+  "result";
+]
+
+let names_0x7f2c2b61cdf0 = [
+]
+
+let co_0x7f2c2b61cdf0 = {
+  co_code = bc_0x7f2c2b61cdf0;
+  co_consts = consts_0x7f2c2b61cdf0;
+  co_varnames = varnames_0x7f2c2b61cdf0;
+  co_names = names_0x7f2c2b61cdf0
+}
+
+let virt_m, res = runCode_returnVM co_0x7f2c2b61cdf0
 let print_program_state = IO.print_string (print_program_state virt_m res)
